theories/sessiontypes/langlemmas.v
@@ -2,110 +2,34 @@ From iris.proofmode Require Export tactics.
 Require Export diris.sessiontypes.langdef.
 Require Export diris.sessiontypes.rtypesystem.
 
-Lemma Γunrestricted_empty : Γunrestricted ∅.
+Lemma subst_rtyped0 (x : string) (v : val) (vT : type) (e : expr) (eT : type) :
+  val_typed v vT -∗
+  rtyped {[ x := vT ]} e eT -∗
+  rtyped0 (subst x v e) eT.
 Proof.
-  intros ??. rewrite lookup_empty. intros. simplify_eq.
-Qed.
-
-Lemma pure_step_rtyped e e' t :
-  pure_step e e' -> rtyped ∅ e t -∗ rtyped ∅ e' t.
-Proof.
-  intros Hps.
-  iIntros "Ht".
-  iInduction Hps as [] "IH"; simpl.
-  - iDestruct "Ht" as (t1 t2 Γ1 Γ2 [-> [HH Hdisj]]) "Ht".
-    iDestruct "Ht" as "((_ & Ht1) & (_ & Ht2))".
-    iSplit. { iPureIntro. apply Γunrestricted_empty. }
-    iExists _,_.
-    iSplit; first done.
-    iFrame.
-  - iDestruct "Ht" as (t1 t2 -> ?) "Ht". eauto.
-  - iDestruct "Ht" as (t' Γ1 Γ2 H) "Ht".
-    iDestruct "Ht" as "((_ & Ht1) & (_ & Ht2))".
-    iDestruct "Ht1" as (t1 t2 HH) "Ht1".
-    simplify_eq.
-    replace (∅ : envT) with (delete x {[ x:= t1 ]} : envT) by (by rewrite delete_singleton).
-    iApply (subst_rtyped with "Ht2 Ht1").
-    rewrite lookup_singleton. done.
-  - iDestruct "Ht" as (t' Γ1 Γ2 H) "Ht".
-    iDestruct "Ht" as "((_ & Ht1) & (_ & Ht2))".
-    iDestruct "Ht1" as (t1 t2 HH) "Ht1".
-    simplify_eq.
-    replace (∅ : envT) with (delete x {[ x:= t1 ]} : envT) by (by rewrite delete_singleton).
-    iApply (subst_rtyped with "Ht2 Ht1").
-    rewrite lookup_singleton. done.
-  - iSplit; first done.
-    iDestruct "Ht" as (t1 t2 [-> _]) "Ht".
-    iExists _,_.
-    iSplit; first done. rewrite left_id. done.
-  - iSplit; first done.
-    iDestruct "Ht" as (t1 t2 [-> _]) "Ht".
-    iExists _,_.
-    iSplit; first done. rewrite left_id. done.
-  - iDestruct "Ht" as (Γ1 Γ2 HH) "[_ [Ht _]]".
-    assert (Γ2 = ∅).
-    { destruct HH. symmetry in H0.
-      assert (Γ1 = ∅). eapply map_positive_l; done. subst.
-      rewrite left_id in H0. done. }
-    subst. done.
-  - iDestruct "Ht" as (Γ1 Γ2 H) "[_ [_ Ht]]".
-    assert (Γ2 = ∅).
-    { destruct H. symmetry in H.
-      assert (Γ1 = ∅). eapply map_positive_l; done. subst.
-      rewrite left_id in H. done. }
-    subst. done.
-  - iDestruct "Ht" as (t1 t2 Γ1 Γ2 (H & Hdisj & Hx)) "[[% Hv] Ht]".
-    eapply both_emp in H as [-> ->].
-    iDestruct "Hv" as (t0 t3 HH) "Hv". simplify_eq.
-    rewrite !left_id.
-    destruct b.
-    + replace (∅ : envT) with (delete x {[ x := t0]} : envT); last first.
-      { apply delete_singleton. }
-      iDestruct "Ht" as "[Ht _]".
-      iApply (subst_rtyped with "Hv Ht").
-      rewrite lookup_singleton //.
-    + replace (∅ : envT) with (delete x {[ x := t3]} : envT); last first.
-      { apply delete_singleton. }
-      iDestruct "Ht" as "[_ Ht]".
-      iApply (subst_rtyped with "Hv Ht").
-      rewrite lookup_singleton //.
-  - iDestruct "Ht" as (t' Γ1 Γ2 H) "[[% Hv] Ht]".
-    destruct H as (H & _ & _).
-    subst. symmetry in H.
-    assert (Γ1 = ∅) as ->. { by eapply map_positive_l. }
-    rewrite left_id_L in H. subst. rewrite left_id_L.
-    replace (∅ : envT) with (delete x {[ x := t']} : envT); last first.
-    { apply delete_singleton. }
-    iApply (subst_rtyped with "Hv Ht").
-    rewrite lookup_singleton. done.
-  - iDestruct "Ht" as (Γ1 Γ2 (H & Hd)) "[% Ht]".
-    destruct H0.
-    symmetry in H.
-    assert (Γ1 = ∅) as ->. { by eapply map_positive_l. }
-    rewrite left_id_L in H. subst. done.
-  - iDestruct "Ht" as (t1 t2 Γ1 Γ2 (? & ? & ? & ?)) "[[% Hv] Ht]".
-    iDestruct "Hv" as (t1' t2' HH) "[Hv1 Hv2]".
-    simplify_eq.
-    symmetry in H0.
-    assert (Γ1 = ∅) as ->. { by eapply map_positive_l. }
-    rewrite left_id_L in H0. subst.
-    rewrite left_id.
-    replace (∅ : envT) with (delete x1 $ delete x2 $ ({[x1 := t1']} ∪ {[x2 := t2']}) : envT); last first.
-    { rewrite delete_union delete_singleton right_id.
-      rewrite delete_singleton_ne; eauto.
-      apply delete_singleton. }
-    iApply (subst_rtyped with "Hv1 [Ht Hv2]").
-    + rewrite delete_union delete_singleton right_id.
-      rewrite delete_singleton_ne; eauto. rewrite lookup_singleton. done.
-    + iApply (subst_rtyped with "Hv2 Ht").
-      rewrite lookup_union lookup_singleton lookup_singleton_ne; eauto.
+  iIntros "Hv Hr".
+  rewrite -rtyped_rtyped0_iff.
+  replace (∅ : envT) with (delete x {[ x := vT]} : envT) by (apply delete_singleton).
+  iApply (subst_rtyped with "Hv Hr"). rewrite lookup_singleton //.
 Qed.
 
 Lemma pure_step_rtyped0 e e' t :
   pure_step e e' -> rtyped0 e t -∗ rtyped0 e' t.
 Proof.
-  iIntros (Hs) "Ht".
-  iApply rtyped_rtyped0.
-  iDestruct (rtyped0_rtyped with "Ht") as "Ht".
-  iApply (pure_step_rtyped with "Ht"). done.
+  intros Hps.
+  iIntros "Ht".
+  iInduction Hps as [] "IH"; simpl;
+  repeat (iDestruct "Ht" as "[Ht Ht2]" || iDestruct "Ht" as (?) "Ht"); eauto; try destruct b; simplify_eq;
+  try iApply (subst_rtyped0 with "Ht2 Ht");
+  try solve [try iDestruct "Ht2" as "[_ Ht2]"; eauto; try iApply (subst_rtyped0 with "Ht Ht2")];
+  try solve [try iDestruct "Ht2" as "[Ht2 _]"; eauto; try iApply (subst_rtyped0 with "Ht Ht2")].
+  iDestruct "Ht" as "%".
+  iDestruct "Ht2" as "[Ht2 HH]".
+  iDestruct "Ht2" as (t0 t3 HH) "[Hv1 Hv2]".
+  rewrite -rtyped_rtyped0_iff.
+  replace (∅ : envT) with (delete x1 $ delete x2 $ (({[x1 := t1]} ∪ {[x2 := t2]})) : envT); last first.
+  { rewrite delete_union delete_singleton right_id delete_singleton_ne // delete_singleton //. }
+  iApply (subst_rtyped with "Hv1 [HH Hv2]"); simplify_eq.
+  + rewrite delete_union delete_singleton right_id delete_singleton_ne // lookup_singleton //.
+  + iApply (subst_rtyped with "Hv2 HH"). rewrite lookup_union lookup_singleton lookup_singleton_ne //.
 Qed.
